Challenge/Bls12381G1Add/Reference/Proofs/FrozenBlock.lean
@@ -16,197 +16,173 @@ open YulSemantics.EVM (Op)
 def frozenReferenceBlock : Block Op :=
 [YulSemantics.Stmt.funDef
    "\x000"
-   ["\x0013", "\x0014"]
-   ["\x0015"]
+   ["\x0016", "\x0017"]
+   ["\x0018"]
    [YulSemantics.Stmt.letDecl
-      ["\x0016"]
+      ["\x0019"]
       (some (YulSemantics.Expr.lit (YulSemantics.Literal.number 34565483545414906068789196026815425751))),
     YulSemantics.Stmt.letDecl
-      ["\x0017"]
+      ["\x0020"]
       (some (YulSemantics.Expr.lit
          (YulSemantics.Literal.number 45442060874369865957053122457065728162598490762543039060009208264153100167851))),
     YulSemantics.Stmt.assign
-      ["\x0015"]
+      ["\x0018"]
       (YulSemantics.Expr.builtin
         (YulSemantics.EVM.Op.or)
         [YulSemantics.Expr.builtin
            (YulSemantics.EVM.Op.gt)
-           [YulSemantics.Expr.var "\x0013", YulSemantics.Expr.var "\x0016"],
+           [YulSemantics.Expr.var "\x0016", YulSemantics.Expr.var "\x0019"],
          YulSemantics.Expr.builtin
            (YulSemantics.EVM.Op.and)
            [YulSemantics.Expr.builtin
               (YulSemantics.EVM.Op.eq)
-              [YulSemantics.Expr.var "\x0013", YulSemantics.Expr.var "\x0016"],
+              [YulSemantics.Expr.var "\x0016", YulSemantics.Expr.var "\x0019"],
             YulSemantics.Expr.builtin
               (YulSemantics.EVM.Op.iszero)
               [YulSemantics.Expr.builtin
                  (YulSemantics.EVM.Op.lt)
-                 [YulSemantics.Expr.var "\x0014", YulSemantics.Expr.var "\x0017"]]]])],
+                 [YulSemantics.Expr.var "\x0017", YulSemantics.Expr.var "\x0020"]]]])],
  YulSemantics.Stmt.funDef
    "\x001"
-   ["\x0018", "\x0019"]
-   ["\x0020"]
-   [YulSemantics.Stmt.assign
-      ["\x0020"]
-      (YulSemantics.Expr.builtin
-        (YulSemantics.EVM.Op.iszero)
-        [YulSemantics.Expr.call "\x000" [YulSemantics.Expr.var "\x0018", YulSemantics.Expr.var "\x0019"]])],
- YulSemantics.Stmt.funDef
-   "\x002"
    ["\x0021", "\x0022"]
    ["\x0023"]
    [YulSemantics.Stmt.assign
       ["\x0023"]
       (YulSemantics.Expr.builtin
+        (YulSemantics.EVM.Op.iszero)
+        [YulSemantics.Expr.call "\x000" [YulSemantics.Expr.var "\x0021", YulSemantics.Expr.var "\x0022"]])],
+ YulSemantics.Stmt.funDef
+   "\x002"
+   ["\x0024", "\x0025"]
+   ["\x0026"]
+   [YulSemantics.Stmt.assign
+      ["\x0026"]
+      (YulSemantics.Expr.builtin
         (YulSemantics.EVM.Op.and)
-        [YulSemantics.Expr.builtin (YulSemantics.EVM.Op.iszero) [YulSemantics.Expr.var "\x0021"],
-         YulSemantics.Expr.builtin (YulSemantics.EVM.Op.iszero) [YulSemantics.Expr.var "\x0022"]])],
+        [YulSemantics.Expr.builtin (YulSemantics.EVM.Op.iszero) [YulSemantics.Expr.var "\x0024"],
+         YulSemantics.Expr.builtin (YulSemantics.EVM.Op.iszero) [YulSemantics.Expr.var "\x0025"]])],
  YulSemantics.Stmt.funDef
    "\x003"
-   ["\x0024", "\x0025", "\x0026", "\x0027"]
-   ["\x0028"]
+   ["\x0027", "\x0028", "\x0029", "\x0030"]
+   ["\x0031"]
    [YulSemantics.Stmt.assign
-      ["\x0028"]
+      ["\x0031"]
       (YulSemantics.Expr.builtin
         (YulSemantics.EVM.Op.and)
         [YulSemantics.Expr.builtin
            (YulSemantics.EVM.Op.eq)
-           [YulSemantics.Expr.var "\x0024", YulSemantics.Expr.var "\x0026"],
+           [YulSemantics.Expr.var "\x0027", YulSemantics.Expr.var "\x0029"],
          YulSemantics.Expr.builtin
            (YulSemantics.EVM.Op.eq)
-           [YulSemantics.Expr.var "\x0025", YulSemantics.Expr.var "\x0027"]])],
+           [YulSemantics.Expr.var "\x0028", YulSemantics.Expr.var "\x0030"]])],
  YulSemantics.Stmt.funDef
    "\x004"
-   ["\x0029", "\x0030", "\x0031", "\x0032"]
-   ["\x0033", "\x0034"]
+   ["\x0032", "\x0033", "\x0034", "\x0035"]
+   ["\x0036", "\x0037"]
    [YulSemantics.Stmt.assign
-      ["\x0034"]
+      ["\x0037"]
       (YulSemantics.Expr.builtin
         (YulSemantics.EVM.Op.add)
-        [YulSemantics.Expr.var "\x0030", YulSemantics.Expr.var "\x0032"]),
+        [YulSemantics.Expr.var "\x0033", YulSemantics.Expr.var "\x0035"]),
     YulSemantics.Stmt.assign
-      ["\x0033"]
+      ["\x0036"]
       (YulSemantics.Expr.builtin
         (YulSemantics.EVM.Op.add)
         [YulSemantics.Expr.builtin
            (YulSemantics.EVM.Op.add)
-           [YulSemantics.Expr.var "\x0029", YulSemantics.Expr.var "\x0031"],
+           [YulSemantics.Expr.var "\x0032", YulSemantics.Expr.var "\x0034"],
          YulSemantics.Expr.builtin
            (YulSemantics.EVM.Op.lt)
-           [YulSemantics.Expr.var "\x0034", YulSemantics.Expr.var "\x0030"]]),
+           [YulSemantics.Expr.var "\x0037", YulSemantics.Expr.var "\x0033"]]),
     YulSemantics.Stmt.cond
-      (YulSemantics.Expr.call "\x000" [YulSemantics.Expr.var "\x0033", YulSemantics.Expr.var "\x0034"])
+      (YulSemantics.Expr.call "\x000" [YulSemantics.Expr.var "\x0036", YulSemantics.Expr.var "\x0037"])
       [YulSemantics.Stmt.letDecl
-         ["\x0035"]
+         ["\x0038"]
          (some (YulSemantics.Expr.lit (YulSemantics.Literal.number 34565483545414906068789196026815425751))),
        YulSemantics.Stmt.letDecl
-         ["\x0036"]
+         ["\x0039"]
          (some (YulSemantics.Expr.lit
             (YulSemantics.Literal.number
               45442060874369865957053122457065728162598490762543039060009208264153100167851))),
        YulSemantics.Stmt.letDecl
-         ["\x0037"]
+         ["\x0040"]
          (some (YulSemantics.Expr.builtin
             (YulSemantics.EVM.Op.sub)
-            [YulSemantics.Expr.var "\x0034", YulSemantics.Expr.var "\x0036"])),
+            [YulSemantics.Expr.var "\x0037", YulSemantics.Expr.var "\x0039"])),
        YulSemantics.Stmt.assign
-         ["\x0033"]
+         ["\x0036"]
          (YulSemantics.Expr.builtin
            (YulSemantics.EVM.Op.sub)
-           [YulSemantics.Expr.var "\x0033",
+           [YulSemantics.Expr.var "\x0036",
             YulSemantics.Expr.builtin
               (YulSemantics.EVM.Op.add)
-              [YulSemantics.Expr.var "\x0035",
+              [YulSemantics.Expr.var "\x0038",
                YulSemantics.Expr.builtin
                  (YulSemantics.EVM.Op.gt)
-                 [YulSemantics.Expr.var "\x0036", YulSemantics.Expr.var "\x0034"]]]),
-       YulSemantics.Stmt.assign ["\x0034"] (YulSemantics.Expr.var "\x0037")]],
+                 [YulSemantics.Expr.var "\x0039", YulSemantics.Expr.var "\x0037"]]]),
+       YulSemantics.Stmt.assign ["\x0037"] (YulSemantics.Expr.var "\x0040")]],
  YulSemantics.Stmt.funDef
    "\x005"
-   ["\x0038", "\x0039", "\x0040", "\x0041"]
-   ["\x0042", "\x0043"]
+   ["\x0041", "\x0042", "\x0043", "\x0044"]
+   ["\x0045", "\x0046"]
    [YulSemantics.Stmt.assign
-      ["\x0043"]
+      ["\x0046"]
       (YulSemantics.Expr.builtin
         (YulSemantics.EVM.Op.sub)
-        [YulSemantics.Expr.var "\x0039", YulSemantics.Expr.var "\x0041"]),
+        [YulSemantics.Expr.var "\x0042", YulSemantics.Expr.var "\x0044"]),
     YulSemantics.Stmt.assign
-      ["\x0042"]
+      ["\x0045"]
       (YulSemantics.Expr.builtin
         (YulSemantics.EVM.Op.sub)
         [YulSemantics.Expr.builtin
            (YulSemantics.EVM.Op.sub)
-           [YulSemantics.Expr.var "\x0038", YulSemantics.Expr.var "\x0040"],
+           [YulSemantics.Expr.var "\x0041", YulSemantics.Expr.var "\x0043"],
          YulSemantics.Expr.builtin
            (YulSemantics.EVM.Op.gt)
-           [YulSemantics.Expr.var "\x0041", YulSemantics.Expr.var "\x0039"]]),
+           [YulSemantics.Expr.var "\x0044", YulSemantics.Expr.var "\x0042"]]),
     YulSemantics.Stmt.letDecl
-      ["\x0044"]
+      ["\x0047"]
       (some (YulSemantics.Expr.lit (YulSemantics.Literal.number 34565483545414906068789196026815425751))),
     YulSemantics.Stmt.cond
       (YulSemantics.Expr.builtin
         (YulSemantics.EVM.Op.gt)
-        [YulSemantics.Expr.var "\x0042", YulSemantics.Expr.var "\x0044"])
+        [YulSemantics.Expr.var "\x0045", YulSemantics.Expr.var "\x0047"])
       [YulSemantics.Stmt.letDecl
-         ["\x0045"]
+         ["\x0048"]
          (some (YulSemantics.Expr.lit
             (YulSemantics.Literal.number
               45442060874369865957053122457065728162598490762543039060009208264153100167851))),
        YulSemantics.Stmt.letDecl
-         ["\x0046"]
+         ["\x0049"]
          (some (YulSemantics.Expr.builtin
             (YulSemantics.EVM.Op.add)
-            [YulSemantics.Expr.var "\x0043", YulSemantics.Expr.var "\x0045"])),
+            [YulSemantics.Expr.var "\x0046", YulSemantics.Expr.var "\x0048"])),
        YulSemantics.Stmt.assign
-         ["\x0042"]
+         ["\x0045"]
          (YulSemantics.Expr.builtin
            (YulSemantics.EVM.Op.add)
            [YulSemantics.Expr.builtin
               (YulSemantics.EVM.Op.add)
-              [YulSemantics.Expr.var "\x0042", YulSemantics.Expr.var "\x0044"],
+              [YulSemantics.Expr.var "\x0045", YulSemantics.Expr.var "\x0047"],
             YulSemantics.Expr.builtin
               (YulSemantics.EVM.Op.lt)
-              [YulSemantics.Expr.var "\x0046", YulSemantics.Expr.var "\x0043"]]),
-       YulSemantics.Stmt.assign ["\x0043"] (YulSemantics.Expr.var "\x0046")]],
+              [YulSemantics.Expr.var "\x0049", YulSemantics.Expr.var "\x0046"]]),
+       YulSemantics.Stmt.assign ["\x0046"] (YulSemantics.Expr.var "\x0049")]],
  YulSemantics.Stmt.funDef
    "\x006"
-   ["\x0047", "\x0048", "\x0049", "\x0050"]
-   ["\x0051", "\x0052", "\x0053"]
+   ["\x0050", "\x0051", "\x0052", "\x0053"]
+   ["\x0054", "\x0055", "\x0056"]
    [YulSemantics.Stmt.assign
-      ["\x0053"]
+      ["\x0056"]
       (YulSemantics.Expr.builtin
         (YulSemantics.EVM.Op.mul)
-        [YulSemantics.Expr.var "\x0048", YulSemantics.Expr.var "\x0050"]),
-    YulSemantics.Stmt.letDecl
-      ["\x0054"]
-      (some (YulSemantics.Expr.builtin
-         (YulSemantics.EVM.Op.mulmod)
-         [YulSemantics.Expr.var "\x0048",
-          YulSemantics.Expr.var "\x0050",
-          YulSemantics.Expr.builtin
-            (YulSemantics.EVM.Op.not)
-            [YulSemantics.Expr.lit (YulSemantics.Literal.number 0)]])),
-    YulSemantics.Stmt.letDecl
-      ["\x0055"]
-      (some (YulSemantics.Expr.builtin
-         (YulSemantics.EVM.Op.sub)
-         [YulSemantics.Expr.builtin
-            (YulSemantics.EVM.Op.sub)
-            [YulSemantics.Expr.var "\x0054", YulSemantics.Expr.var "\x0053"],
-          YulSemantics.Expr.builtin
-            (YulSemantics.EVM.Op.lt)
-            [YulSemantics.Expr.var "\x0054", YulSemantics.Expr.var "\x0053"]])),
-    YulSemantics.Stmt.letDecl
-      ["\x0056"]
-      (some (YulSemantics.Expr.builtin
-         (YulSemantics.EVM.Op.mul)
-         [YulSemantics.Expr.var "\x0047", YulSemantics.Expr.var "\x0050"])),
+        [YulSemantics.Expr.var "\x0051", YulSemantics.Expr.var "\x0053"]),
     YulSemantics.Stmt.letDecl
       ["\x0057"]
       (some (YulSemantics.Expr.builtin
          (YulSemantics.EVM.Op.mulmod)
-         [YulSemantics.Expr.var "\x0047",
-          YulSemantics.Expr.var "\x0050",
+         [YulSemantics.Expr.var "\x0051",
+          YulSemantics.Expr.var "\x0053",
           YulSemantics.Expr.builtin
             (YulSemantics.EVM.Op.not)
             [YulSemantics.Expr.lit (YulSemantics.Literal.number 0)]])),
@@ -224,13 +200,13 @@ def frozenReferenceBlock : Block Op :=
       ["\x0059"]
       (some (YulSemantics.Expr.builtin
          (YulSemantics.EVM.Op.mul)
-         [YulSemantics.Expr.var "\x0048", YulSemantics.Expr.var "\x0049"])),
+         [YulSemantics.Expr.var "\x0050", YulSemantics.Expr.var "\x0053"])),
     YulSemantics.Stmt.letDecl
       ["\x0060"]
       (some (YulSemantics.Expr.builtin
          (YulSemantics.EVM.Op.mulmod)
-         [YulSemantics.Expr.var "\x0048",
-          YulSemantics.Expr.var "\x0049",
+         [YulSemantics.Expr.var "\x0050",
+          YulSemantics.Expr.var "\x0053",
           YulSemantics.Expr.builtin
             (YulSemantics.EVM.Op.not)
             [YulSemantics.Expr.lit (YulSemantics.Literal.number 0)]])),
@@ -244,268 +220,1064 @@ def frozenReferenceBlock : Block Op :=
           YulSemantics.Expr.builtin
             (YulSemantics.EVM.Op.lt)
             [YulSemantics.Expr.var "\x0060", YulSemantics.Expr.var "\x0059"]])),
-    YulSemantics.Stmt.assign
-      ["\x0052"]
-      (YulSemantics.Expr.builtin
-        (YulSemantics.EVM.Op.add)
-        [YulSemantics.Expr.var "\x0055", YulSemantics.Expr.var "\x0056"]),
     YulSemantics.Stmt.letDecl
       ["\x0062"]
       (some (YulSemantics.Expr.builtin
-         (YulSemantics.EVM.Op.lt)
-         [YulSemantics.Expr.var "\x0052", YulSemantics.Expr.var "\x0055"])),
+         (YulSemantics.EVM.Op.mul)
+         [YulSemantics.Expr.var "\x0051", YulSemantics.Expr.var "\x0052"])),
     YulSemantics.Stmt.letDecl
       ["\x0063"]
       (some (YulSemantics.Expr.builtin
-         (YulSemantics.EVM.Op.add)
-         [YulSemantics.Expr.var "\x0052", YulSemantics.Expr.var "\x0059"])),
+         (YulSemantics.EVM.Op.mulmod)
+         [YulSemantics.Expr.var "\x0051",
+          YulSemantics.Expr.var "\x0052",
+          YulSemantics.Expr.builtin
+            (YulSemantics.EVM.Op.not)
+            [YulSemantics.Expr.lit (YulSemantics.Literal.number 0)]])),
+    YulSemantics.Stmt.letDecl
+      ["\x0064"]
+      (some (YulSemantics.Expr.builtin
+         (YulSemantics.EVM.Op.sub)
+         [YulSemantics.Expr.builtin
+            (YulSemantics.EVM.Op.sub)
+            [YulSemantics.Expr.var "\x0063", YulSemantics.Expr.var "\x0062"],
+          YulSemantics.Expr.builtin
+            (YulSemantics.EVM.Op.lt)
+            [YulSemantics.Expr.var "\x0063", YulSemantics.Expr.var "\x0062"]])),
     YulSemantics.Stmt.assign
-      ["\x0062"]
+      ["\x0055"]
       (YulSemantics.Expr.builtin
         (YulSemantics.EVM.Op.add)
-        [YulSemantics.Expr.var "\x0062",
+        [YulSemantics.Expr.var "\x0058", YulSemantics.Expr.var "\x0059"]),
+    YulSemantics.Stmt.letDecl
+      ["\x0065"]
+      (some (YulSemantics.Expr.builtin
+         (YulSemantics.EVM.Op.lt)
+         [YulSemantics.Expr.var "\x0055", YulSemantics.Expr.var "\x0058"])),
+    YulSemantics.Stmt.letDecl
+      ["\x0066"]
+      (some (YulSemantics.Expr.builtin
+         (YulSemantics.EVM.Op.add)
+         [YulSemantics.Expr.var "\x0055", YulSemantics.Expr.var "\x0062"])),
+    YulSemantics.Stmt.assign
+      ["\x0065"]
+      (YulSemantics.Expr.builtin
+        (YulSemantics.EVM.Op.add)
+        [YulSemantics.Expr.var "\x0065",
          YulSemantics.Expr.builtin
            (YulSemantics.EVM.Op.lt)
-           [YulSemantics.Expr.var "\x0063", YulSemantics.Expr.var "\x0052"]]),
-    YulSemantics.Stmt.assign ["\x0052"] (YulSemantics.Expr.var "\x0063"),
+           [YulSemantics.Expr.var "\x0066", YulSemantics.Expr.var "\x0055"]]),
+    YulSemantics.Stmt.assign ["\x0055"] (YulSemantics.Expr.var "\x0066"),
     YulSemantics.Stmt.assign
-      ["\x0051"]
+      ["\x0054"]
       (YulSemantics.Expr.builtin
         (YulSemantics.EVM.Op.add)
         [YulSemantics.Expr.builtin
            (YulSemantics.EVM.Op.add)
-           [YulSemantics.Expr.var "\x0058", YulSemantics.Expr.var "\x0061"],
+           [YulSemantics.Expr.var "\x0061", YulSemantics.Expr.var "\x0064"],
          YulSemantics.Expr.builtin
            (YulSemantics.EVM.Op.add)
            [YulSemantics.Expr.builtin
               (YulSemantics.EVM.Op.mul)
-              [YulSemantics.Expr.var "\x0047", YulSemantics.Expr.var "\x0049"],
-            YulSemantics.Expr.var "\x0062"]])],
+              [YulSemantics.Expr.var "\x0050", YulSemantics.Expr.var "\x0052"],
+            YulSemantics.Expr.var "\x0065"]])],
  YulSemantics.Stmt.funDef
    "\x007"
-   ["\x0064", "\x0065", "\x0066"]
+   ["\x0067", "\x0068", "\x0069"]
    []
    [YulSemantics.Stmt.exprStmt
       (YulSemantics.Expr.builtin
         (YulSemantics.EVM.Op.mstore)
-        [YulSemantics.Expr.var "\x0064",
+        [YulSemantics.Expr.var "\x0067",
          YulSemantics.Expr.builtin
            (YulSemantics.EVM.Op.shl)
-           [YulSemantics.Expr.lit (YulSemantics.Literal.number 128), YulSemantics.Expr.var "\x0065"]]),
+           [YulSemantics.Expr.lit (YulSemantics.Literal.number 128), YulSemantics.Expr.var "\x0068"]]),
     YulSemantics.Stmt.exprStmt
       (YulSemantics.Expr.builtin
         (YulSemantics.EVM.Op.mstore)
         [YulSemantics.Expr.builtin
            (YulSemantics.EVM.Op.add)
-           [YulSemantics.Expr.var "\x0064", YulSemantics.Expr.lit (YulSemantics.Literal.number 16)],
-         YulSemantics.Expr.var "\x0066"])],
+           [YulSemantics.Expr.var "\x0067", YulSemantics.Expr.lit (YulSemantics.Literal.number 16)],
+         YulSemantics.Expr.var "\x0069"])],
  YulSemantics.Stmt.funDef
    "\x008"
-   ["\x0067"]
+   ["\x0070"]
    []
    [YulSemantics.Stmt.exprStmt
       (YulSemantics.Expr.call
         "\x007"
-        [YulSemantics.Expr.var "\x0067",
+        [YulSemantics.Expr.var "\x0070",
          YulSemantics.Expr.lit (YulSemantics.Literal.number 34565483545414906068789196026815425751),
          YulSemantics.Expr.lit
            (YulSemantics.Literal.number
              45442060874369865957053122457065728162598490762543039060009208264153100167851)])],
  YulSemantics.Stmt.funDef
    "\x009"
-   ["\x0068", "\x0069", "\x0070", "\x0071"]
-   ["\x0072", "\x0073"]
+   ["\x0071", "\x0072", "\x0073", "\x0074"]
+   ["\x0075", "\x0076"]
    [YulSemantics.Stmt.letDecl
-      ["\x0074", "\x0075", "\x0076"]
+      ["\x0077", "\x0078", "\x0079"]
       (some (YulSemantics.Expr.call
          "\x006"
-         [YulSemantics.Expr.var "\x0068",
-          YulSemantics.Expr.var "\x0069",
-          YulSemantics.Expr.var "\x0070",
-          YulSemantics.Expr.var "\x0071"])),
-    YulSemantics.Stmt.exprStmt
-      (YulSemantics.Expr.builtin
-        (YulSemantics.EVM.Op.mstore)
-        [YulSemantics.Expr.lit (YulSemantics.Literal.number 1024),
-         YulSemantics.Expr.lit (YulSemantics.Literal.number 96)]),
-    YulSemantics.Stmt.exprStmt
-      (YulSemantics.Expr.builtin
-        (YulSemantics.EVM.Op.mstore)
-        [YulSemantics.Expr.lit (YulSemantics.Literal.number 1056),
-         YulSemantics.Expr.lit (YulSemantics.Literal.number 1)]),
-    YulSemantics.Stmt.exprStmt
-      (YulSemantics.Expr.builtin
-        (YulSemantics.EVM.Op.mstore)
-        [YulSemantics.Expr.lit (YulSemantics.Literal.number 1088),
-         YulSemantics.Expr.lit (YulSemantics.Literal.number 48)]),
-    YulSemantics.Stmt.exprStmt
-      (YulSemantics.Expr.builtin
-        (YulSemantics.EVM.Op.mstore)
-        [YulSemantics.Expr.lit (YulSemantics.Literal.number 1120), YulSemantics.Expr.var "\x0074"]),
-    YulSemantics.Stmt.exprStmt
-      (YulSemantics.Expr.builtin
-        (YulSemantics.EVM.Op.mstore)
-        [YulSemantics.Expr.lit (YulSemantics.Literal.number 1152), YulSemantics.Expr.var "\x0075"]),
-    YulSemantics.Stmt.exprStmt
-      (YulSemantics.Expr.builtin
-        (YulSemantics.EVM.Op.mstore)
-        [YulSemantics.Expr.lit (YulSemantics.Literal.number 1184), YulSemantics.Expr.var "\x0076"]),
-    YulSemantics.Stmt.exprStmt
-      (YulSemantics.Expr.builtin
-        (YulSemantics.EVM.Op.mstore8)
-        [YulSemantics.Expr.lit (YulSemantics.Literal.number 1216),
-         YulSemantics.Expr.lit (YulSemantics.Literal.number 1)]),
-    YulSemantics.Stmt.exprStmt
-      (YulSemantics.Expr.call "\x008" [YulSemantics.Expr.lit (YulSemantics.Literal.number 1217)]),
-    YulSemantics.Stmt.cond
-      (YulSemantics.Expr.builtin
-        (YulSemantics.EVM.Op.iszero)
-        [YulSemantics.Expr.builtin
-           (YulSemantics.EVM.Op.staticcall)
-           [YulSemantics.Expr.lit (YulSemantics.Literal.number 500),
-            YulSemantics.Expr.lit (YulSemantics.Literal.number 5),
-            YulSemantics.Expr.lit (YulSemantics.Literal.number 1024),
-            YulSemantics.Expr.lit (YulSemantics.Literal.number 241),
-            YulSemantics.Expr.lit (YulSemantics.Literal.number 1280),
-            YulSemantics.Expr.lit (YulSemantics.Literal.number 48)]])
-      [YulSemantics.Stmt.exprStmt (YulSemantics.Expr.builtin (YulSemantics.EVM.Op.invalid) [])],
+         [YulSemantics.Expr.var "\x0071",
+          YulSemantics.Expr.var "\x0072",
+          YulSemantics.Expr.var "\x0073",
+          YulSemantics.Expr.var "\x0074"])),
     YulSemantics.Stmt.assign
-      ["\x0072"]
-      (YulSemantics.Expr.builtin
-        (YulSemantics.EVM.Op.shr)
-        [YulSemantics.Expr.lit (YulSemantics.Literal.number 128),
-         YulSemantics.Expr.builtin
-           (YulSemantics.EVM.Op.mload)
-           [YulSemantics.Expr.lit (YulSemantics.Literal.number 1280)]]),
-    YulSemantics.Stmt.assign
-      ["\x0073"]
-      (YulSemantics.Expr.builtin
-        (YulSemantics.EVM.Op.mload)
-        [YulSemantics.Expr.lit (YulSemantics.Literal.number 1296)])],
+      ["\x0075", "\x0076"]
+      (YulSemantics.Expr.call
+        "\x0014"
+        [YulSemantics.Expr.var "\x0077", YulSemantics.Expr.var "\x0078", YulSemantics.Expr.var "\x0079"])],
  YulSemantics.Stmt.funDef
    "\x0010"
-   ["\x0077", "\x0078"]
-   ["\x0079", "\x0080"]
-   [YulSemantics.Stmt.exprStmt
-      (YulSemantics.Expr.builtin
-        (YulSemantics.EVM.Op.mstore)
-        [YulSemantics.Expr.lit (YulSemantics.Literal.number 1024),
-         YulSemantics.Expr.lit (YulSemantics.Literal.number 48)]),
-    YulSemantics.Stmt.exprStmt
-      (YulSemantics.Expr.builtin
-        (YulSemantics.EVM.Op.mstore)
-        [YulSemantics.Expr.lit (YulSemantics.Literal.number 1056),
-         YulSemantics.Expr.lit (YulSemantics.Literal.number 48)]),
-    YulSemantics.Stmt.exprStmt
-      (YulSemantics.Expr.builtin
-        (YulSemantics.EVM.Op.mstore)
-        [YulSemantics.Expr.lit (YulSemantics.Literal.number 1088),
-         YulSemantics.Expr.lit (YulSemantics.Literal.number 48)]),
-    YulSemantics.Stmt.exprStmt
-      (YulSemantics.Expr.call
-        "\x007"
-        [YulSemantics.Expr.lit (YulSemantics.Literal.number 1120),
-         YulSemantics.Expr.var "\x0077",
-         YulSemantics.Expr.var "\x0078"]),
-    YulSemantics.Stmt.exprStmt
-      (YulSemantics.Expr.call
-        "\x007"
-        [YulSemantics.Expr.lit (YulSemantics.Literal.number 1168),
-         YulSemantics.Expr.lit (YulSemantics.Literal.number 34565483545414906068789196026815425751),
-         YulSemantics.Expr.lit
-           (YulSemantics.Literal.number
-             45442060874369865957053122457065728162598490762543039060009208264153100167849)]),
-    YulSemantics.Stmt.exprStmt
-      (YulSemantics.Expr.call "\x008" [YulSemantics.Expr.lit (YulSemantics.Literal.number 1216)]),
-    YulSemantics.Stmt.cond
-      (YulSemantics.Expr.builtin
-        (YulSemantics.EVM.Op.iszero)
-        [YulSemantics.Expr.builtin
-           (YulSemantics.EVM.Op.staticcall)
-           [YulSemantics.Expr.lit (YulSemantics.Literal.number 36576),
-            YulSemantics.Expr.lit (YulSemantics.Literal.number 5),
-            YulSemantics.Expr.lit (YulSemantics.Literal.number 1024),
-            YulSemantics.Expr.lit (YulSemantics.Literal.number 240),
-            YulSemantics.Expr.lit (YulSemantics.Literal.number 1280),
-            YulSemantics.Expr.lit (YulSemantics.Literal.number 48)]])
-      [YulSemantics.Stmt.exprStmt (YulSemantics.Expr.builtin (YulSemantics.EVM.Op.invalid) [])],
-    YulSemantics.Stmt.assign
-      ["\x0079"]
-      (YulSemantics.Expr.builtin
-        (YulSemantics.EVM.Op.shr)
-        [YulSemantics.Expr.lit (YulSemantics.Literal.number 128),
-         YulSemantics.Expr.builtin
-           (YulSemantics.EVM.Op.mload)
-           [YulSemantics.Expr.lit (YulSemantics.Literal.number 1280)]]),
-    YulSemantics.Stmt.assign
-      ["\x0080"]
-      (YulSemantics.Expr.builtin
-        (YulSemantics.EVM.Op.mload)
-        [YulSemantics.Expr.lit (YulSemantics.Literal.number 1296)])],
+   ["\x0080", "\x0081"]
+   ["\x0082", "\x0083"]
+   [YulSemantics.Stmt.assign
+      ["\x0082", "\x0083"]
+      (YulSemantics.Expr.call "\x0013" [YulSemantics.Expr.var "\x0080", YulSemantics.Expr.var "\x0081"])],
  YulSemantics.Stmt.funDef
    "\x0011"
-   ["\x0081", "\x0082", "\x0083", "\x0084"]
-   ["\x0085"]
+   ["\x0084", "\x0085", "\x0086", "\x0087"]
+   ["\x0088"]
    [YulSemantics.Stmt.letDecl
-      ["\x0086", "\x0087"]
+      ["\x0089", "\x0090"]
       (some (YulSemantics.Expr.call
          "\x009"
-         [YulSemantics.Expr.var "\x0083",
+         [YulSemantics.Expr.var "\x0086",
+          YulSemantics.Expr.var "\x0087",
+          YulSemantics.Expr.var "\x0086",
+          YulSemantics.Expr.var "\x0087"])),
+    YulSemantics.Stmt.letDecl
+      ["\x0091", "\x0092"]
+      (some (YulSemantics.Expr.call
+         "\x009"
+         [YulSemantics.Expr.var "\x0084",
+          YulSemantics.Expr.var "\x0085",
           YulSemantics.Expr.var "\x0084",
-          YulSemantics.Expr.var "\x0083",
-          YulSemantics.Expr.var "\x0084"])),
+          YulSemantics.Expr.var "\x0085"])),
     YulSemantics.Stmt.letDecl
-      ["\x0088", "\x0089"]
+      ["\x0093", "\x0094"]
       (some (YulSemantics.Expr.call
          "\x009"
-         [YulSemantics.Expr.var "\x0081",
-          YulSemantics.Expr.var "\x0082",
-          YulSemantics.Expr.var "\x0081",
-          YulSemantics.Expr.var "\x0082"])),
-    YulSemantics.Stmt.letDecl
-      ["\x0090", "\x0091"]
-      (some (YulSemantics.Expr.call
-         "\x009"
-         [YulSemantics.Expr.var "\x0088",
-          YulSemantics.Expr.var "\x0089",
-          YulSemantics.Expr.var "\x0081",
-          YulSemantics.Expr.var "\x0082"])),
+         [YulSemantics.Expr.var "\x0091",
+          YulSemantics.Expr.var "\x0092",
+          YulSemantics.Expr.var "\x0084",
+          YulSemantics.Expr.var "\x0085"])),
     YulSemantics.Stmt.assign
-      ["\x0090", "\x0091"]
+      ["\x0093", "\x0094"]
       (YulSemantics.Expr.call
         "\x004"
-        [YulSemantics.Expr.var "\x0090",
-         YulSemantics.Expr.var "\x0091",
+        [YulSemantics.Expr.var "\x0093",
+         YulSemantics.Expr.var "\x0094",
          YulSemantics.Expr.lit (YulSemantics.Literal.number 0),
          YulSemantics.Expr.lit (YulSemantics.Literal.number 4)]),
     YulSemantics.Stmt.assign
-      ["\x0085"]
+      ["\x0088"]
       (YulSemantics.Expr.call
         "\x003"
-        [YulSemantics.Expr.var "\x0086",
-         YulSemantics.Expr.var "\x0087",
+        [YulSemantics.Expr.var "\x0089",
          YulSemantics.Expr.var "\x0090",
-         YulSemantics.Expr.var "\x0091"])],
+         YulSemantics.Expr.var "\x0093",
+         YulSemantics.Expr.var "\x0094"])],
  YulSemantics.Stmt.funDef
    "\x0012"
-   ["\x0092", "\x0093", "\x0094", "\x0095"]
+   ["\x0095", "\x0096", "\x0097", "\x0098"]
    []
    [YulSemantics.Stmt.exprStmt
       (YulSemantics.Expr.builtin
         (YulSemantics.EVM.Op.mstore)
-        [YulSemantics.Expr.lit (YulSemantics.Literal.number 0), YulSemantics.Expr.var "\x0092"]),
+        [YulSemantics.Expr.lit (YulSemantics.Literal.number 0), YulSemantics.Expr.var "\x0095"]),
     YulSemantics.Stmt.exprStmt
       (YulSemantics.Expr.builtin
         (YulSemantics.EVM.Op.mstore)
-        [YulSemantics.Expr.lit (YulSemantics.Literal.number 32), YulSemantics.Expr.var "\x0093"]),
+        [YulSemantics.Expr.lit (YulSemantics.Literal.number 32), YulSemantics.Expr.var "\x0096"]),
     YulSemantics.Stmt.exprStmt
       (YulSemantics.Expr.builtin
         (YulSemantics.EVM.Op.mstore)
-        [YulSemantics.Expr.lit (YulSemantics.Literal.number 64), YulSemantics.Expr.var "\x0094"]),
+        [YulSemantics.Expr.lit (YulSemantics.Literal.number 64), YulSemantics.Expr.var "\x0097"]),
     YulSemantics.Stmt.exprStmt
       (YulSemantics.Expr.builtin
         (YulSemantics.EVM.Op.mstore)
-        [YulSemantics.Expr.lit (YulSemantics.Literal.number 96), YulSemantics.Expr.var "\x0095"])],
+        [YulSemantics.Expr.lit (YulSemantics.Literal.number 96), YulSemantics.Expr.var "\x0098"])],
+ YulSemantics.Stmt.funDef
+   "\x0013"
+   ["\x00123", "\x00124"]
+   ["\x00125", "\x00126"]
+   [YulSemantics.Stmt.letDecl
+      ["\x00127", "\x00128"]
+      (some (YulSemantics.Expr.call
+         "\x0015"
+         [YulSemantics.Expr.var "\x00124",
+          YulSemantics.Expr.var "\x00123",
+          YulSemantics.Expr.lit
+            (YulSemantics.Literal.number 92286679234085438351495039074048687640204382693166976402664901553327635873368),
+          YulSemantics.Expr.lit (YulSemantics.Literal.number 86499536527081971458999430873902347)])),
+    YulSemantics.Stmt.letDecl ["\x00129"] (some (YulSemantics.Expr.var "\x00127")),
+    YulSemantics.Stmt.letDecl ["\x00130"] (some (YulSemantics.Expr.var "\x00128")),
+    YulSemantics.Stmt.forLoop
+      [YulSemantics.Stmt.letDecl ["\x00131"] (some (YulSemantics.Expr.lit (YulSemantics.Literal.number 124)))]
+      (YulSemantics.Expr.builtin
+        (YulSemantics.EVM.Op.gt)
+        [YulSemantics.Expr.var "\x00131", YulSemantics.Expr.lit (YulSemantics.Literal.number 0)])
+      []
+      [YulSemantics.Stmt.assign
+         ["\x00131"]
+         (YulSemantics.Expr.builtin
+           (YulSemantics.EVM.Op.sub)
+           [YulSemantics.Expr.var "\x00131", YulSemantics.Expr.lit (YulSemantics.Literal.number 1)]),
+       YulSemantics.Stmt.assign
+         ["\x00129", "\x00130"]
+         (YulSemantics.Expr.call
+           "\x0015"
+           [YulSemantics.Expr.var "\x00129",
+            YulSemantics.Expr.var "\x00130",
+            YulSemantics.Expr.var "\x00129",
+            YulSemantics.Expr.var "\x00130"]),
+       YulSemantics.Stmt.cond
+         (YulSemantics.Expr.builtin
+           (YulSemantics.EVM.Op.and)
+           [YulSemantics.Expr.builtin
+              (YulSemantics.EVM.Op.shr)
+              [YulSemantics.Expr.var "\x00131",
+               YulSemantics.Expr.lit (YulSemantics.Literal.number 34565483545414906068789196026815425751)],
+            YulSemantics.Expr.lit (YulSemantics.Literal.number 1)])
+         [YulSemantics.Stmt.assign
+            ["\x00129", "\x00130"]
+            (YulSemantics.Expr.call
+              "\x0015"
+              [YulSemantics.Expr.var "\x00129",
+               YulSemantics.Expr.var "\x00130",
+               YulSemantics.Expr.var "\x00127",
+               YulSemantics.Expr.var "\x00128"])]],
+    YulSemantics.Stmt.forLoop
+      [YulSemantics.Stmt.letDecl ["\x00132"] (some (YulSemantics.Expr.lit (YulSemantics.Literal.number 256)))]
+      (YulSemantics.Expr.builtin
+        (YulSemantics.EVM.Op.gt)
+        [YulSemantics.Expr.var "\x00132", YulSemantics.Expr.lit (YulSemantics.Literal.number 0)])
+      []
+      [YulSemantics.Stmt.assign
+         ["\x00132"]
+         (YulSemantics.Expr.builtin
+           (YulSemantics.EVM.Op.sub)
+           [YulSemantics.Expr.var "\x00132", YulSemantics.Expr.lit (YulSemantics.Literal.number 1)]),
+       YulSemantics.Stmt.assign
+         ["\x00129", "\x00130"]
+         (YulSemantics.Expr.call
+           "\x0015"
+           [YulSemantics.Expr.var "\x00129",
+            YulSemantics.Expr.var "\x00130",
+            YulSemantics.Expr.var "\x00129",
+            YulSemantics.Expr.var "\x00130"]),
+       YulSemantics.Stmt.cond
+         (YulSemantics.Expr.builtin
+           (YulSemantics.EVM.Op.and)
+           [YulSemantics.Expr.builtin
+              (YulSemantics.EVM.Op.shr)
+              [YulSemantics.Expr.var "\x00132",
+               YulSemantics.Expr.lit
+                 (YulSemantics.Literal.number
+                   45442060874369865957053122457065728162598490762543039060009208264153100167849)],
+            YulSemantics.Expr.lit (YulSemantics.Literal.number 1)])
+         [YulSemantics.Stmt.assign
+            ["\x00129", "\x00130"]
+            (YulSemantics.Expr.call
+              "\x0015"
+              [YulSemantics.Expr.var "\x00129",
+               YulSemantics.Expr.var "\x00130",
+               YulSemantics.Expr.var "\x00127",
+               YulSemantics.Expr.var "\x00128"])]],
+    YulSemantics.Stmt.assign
+      ["\x00126", "\x00125"]
+      (YulSemantics.Expr.call
+        "\x0015"
+        [YulSemantics.Expr.var "\x00129",
+         YulSemantics.Expr.var "\x00130",
+         YulSemantics.Expr.lit (YulSemantics.Literal.number 1),
+         YulSemantics.Expr.lit (YulSemantics.Literal.number 0)])],
+ YulSemantics.Stmt.funDef
+   "\x0014"
+   ["\x00133", "\x00134", "\x00135"]
+   ["\x00136", "\x00137"]
+   [YulSemantics.Stmt.letDecl ["\x00138"] none,
+    YulSemantics.Stmt.letDecl ["\x00139"] none,
+    YulSemantics.Stmt.block
+      [YulSemantics.Stmt.letDecl
+         ["\x00140"]
+         (some (YulSemantics.Expr.lit
+            (YulSemantics.Literal.number
+              78351685926696084494279172348607765220277164942381371098199816345395397379320))),
+       YulSemantics.Stmt.letDecl
+         ["\x00141"]
+         (some (YulSemantics.Expr.lit
+            (YulSemantics.Literal.number
+              12442938494476872817539570304019263996873168525671286588860177704514606971438))),
+       YulSemantics.Stmt.letDecl
+         ["\x00142"]
+         (some (YulSemantics.Expr.lit (YulSemantics.Literal.number 3349934019733276885328185912087860918825))),
+       YulSemantics.Stmt.letDecl
+         ["\x00143"]
+         (some (YulSemantics.Expr.builtin
+            (YulSemantics.EVM.Op.mul)
+            [YulSemantics.Expr.var "\x00134", YulSemantics.Expr.var "\x00140"])),
+       YulSemantics.Stmt.letDecl
+         ["\x00144"]
+         (some (YulSemantics.Expr.builtin
+            (YulSemantics.EVM.Op.mulmod)
+            [YulSemantics.Expr.var "\x00134",
+             YulSemantics.Expr.var "\x00140",
+             YulSemantics.Expr.builtin
+               (YulSemantics.EVM.Op.not)
+               [YulSemantics.Expr.lit (YulSemantics.Literal.number 0)]])),
+       YulSemantics.Stmt.letDecl
+         ["\x00145"]
+         (some (YulSemantics.Expr.builtin
+            (YulSemantics.EVM.Op.sub)
+            [YulSemantics.Expr.builtin
+               (YulSemantics.EVM.Op.sub)
+               [YulSemantics.Expr.var "\x00144", YulSemantics.Expr.var "\x00143"],
+             YulSemantics.Expr.builtin
+               (YulSemantics.EVM.Op.lt)
+               [YulSemantics.Expr.var "\x00144", YulSemantics.Expr.var "\x00143"]])),
+       YulSemantics.Stmt.letDecl
+         ["\x00146"]
+         (some (YulSemantics.Expr.builtin
+            (YulSemantics.EVM.Op.mul)
+            [YulSemantics.Expr.var "\x00134", YulSemantics.Expr.var "\x00141"])),
+       YulSemantics.Stmt.assign
+         ["\x00144"]
+         (YulSemantics.Expr.builtin
+           (YulSemantics.EVM.Op.mulmod)
+           [YulSemantics.Expr.var "\x00134",
+            YulSemantics.Expr.var "\x00141",
+            YulSemantics.Expr.builtin
+              (YulSemantics.EVM.Op.not)
+              [YulSemantics.Expr.lit (YulSemantics.Literal.number 0)]]),
+       YulSemantics.Stmt.letDecl
+         ["\x00147"]
+         (some (YulSemantics.Expr.builtin
+            (YulSemantics.EVM.Op.sub)
+            [YulSemantics.Expr.builtin
+               (YulSemantics.EVM.Op.sub)
+               [YulSemantics.Expr.var "\x00144", YulSemantics.Expr.var "\x00146"],
+             YulSemantics.Expr.builtin
+               (YulSemantics.EVM.Op.lt)
+               [YulSemantics.Expr.var "\x00144", YulSemantics.Expr.var "\x00146"]])),
+       YulSemantics.Stmt.letDecl
+         ["\x00148"]
+         (some (YulSemantics.Expr.builtin
+            (YulSemantics.EVM.Op.mul)
+            [YulSemantics.Expr.var "\x00134", YulSemantics.Expr.var "\x00142"])),
+       YulSemantics.Stmt.assign
+         ["\x00144"]
+         (YulSemantics.Expr.builtin
+           (YulSemantics.EVM.Op.mulmod)
+           [YulSemantics.Expr.var "\x00134",
+            YulSemantics.Expr.var "\x00142",
+            YulSemantics.Expr.builtin
+              (YulSemantics.EVM.Op.not)
+              [YulSemantics.Expr.lit (YulSemantics.Literal.number 0)]]),
+       YulSemantics.Stmt.letDecl
+         ["\x00149"]
+         (some (YulSemantics.Expr.builtin
+            (YulSemantics.EVM.Op.sub)
+            [YulSemantics.Expr.builtin
+               (YulSemantics.EVM.Op.sub)
+               [YulSemantics.Expr.var "\x00144", YulSemantics.Expr.var "\x00148"],
+             YulSemantics.Expr.builtin
+               (YulSemantics.EVM.Op.lt)
+               [YulSemantics.Expr.var "\x00144", YulSemantics.Expr.var "\x00148"]])),
+       YulSemantics.Stmt.letDecl
+         ["\x00150"]
+         (some (YulSemantics.Expr.builtin
+            (YulSemantics.EVM.Op.mul)
+            [YulSemantics.Expr.var "\x00133", YulSemantics.Expr.var "\x00140"])),
+       YulSemantics.Stmt.assign
+         ["\x00144"]
+         (YulSemantics.Expr.builtin
+           (YulSemantics.EVM.Op.mulmod)
+           [YulSemantics.Expr.var "\x00133",
+            YulSemantics.Expr.var "\x00140",
+            YulSemantics.Expr.builtin
+              (YulSemantics.EVM.Op.not)
+              [YulSemantics.Expr.lit (YulSemantics.Literal.number 0)]]),
+       YulSemantics.Stmt.letDecl
+         ["\x00151"]
+         (some (YulSemantics.Expr.builtin
+            (YulSemantics.EVM.Op.sub)
+            [YulSemantics.Expr.builtin
+               (YulSemantics.EVM.Op.sub)
+               [YulSemantics.Expr.var "\x00144", YulSemantics.Expr.var "\x00150"],
+             YulSemantics.Expr.builtin
+               (YulSemantics.EVM.Op.lt)
+               [YulSemantics.Expr.var "\x00144", YulSemantics.Expr.var "\x00150"]])),
+       YulSemantics.Stmt.letDecl
+         ["\x00152"]
+         (some (YulSemantics.Expr.builtin
+            (YulSemantics.EVM.Op.mul)
+            [YulSemantics.Expr.var "\x00133", YulSemantics.Expr.var "\x00141"])),
+       YulSemantics.Stmt.assign
+         ["\x00144"]
+         (YulSemantics.Expr.builtin
+           (YulSemantics.EVM.Op.mulmod)
+           [YulSemantics.Expr.var "\x00133",
+            YulSemantics.Expr.var "\x00141",
+            YulSemantics.Expr.builtin
+              (YulSemantics.EVM.Op.not)
+              [YulSemantics.Expr.lit (YulSemantics.Literal.number 0)]]),
+       YulSemantics.Stmt.letDecl
+         ["\x00153"]
+         (some (YulSemantics.Expr.builtin
+            (YulSemantics.EVM.Op.sub)
+            [YulSemantics.Expr.builtin
+               (YulSemantics.EVM.Op.sub)
+               [YulSemantics.Expr.var "\x00144", YulSemantics.Expr.var "\x00152"],
+             YulSemantics.Expr.builtin
+               (YulSemantics.EVM.Op.lt)
+               [YulSemantics.Expr.var "\x00144", YulSemantics.Expr.var "\x00152"]])),
+       YulSemantics.Stmt.letDecl
+         ["\x00154"]
+         (some (YulSemantics.Expr.builtin
+            (YulSemantics.EVM.Op.mul)
+            [YulSemantics.Expr.var "\x00133", YulSemantics.Expr.var "\x00142"])),
+       YulSemantics.Stmt.assign
+         ["\x00144"]
+         (YulSemantics.Expr.builtin
+           (YulSemantics.EVM.Op.mulmod)
+           [YulSemantics.Expr.var "\x00133",
+            YulSemantics.Expr.var "\x00142",
+            YulSemantics.Expr.builtin
+              (YulSemantics.EVM.Op.not)
+              [YulSemantics.Expr.lit (YulSemantics.Literal.number 0)]]),
+       YulSemantics.Stmt.letDecl
+         ["\x00155"]
+         (some (YulSemantics.Expr.builtin
+            (YulSemantics.EVM.Op.sub)
+            [YulSemantics.Expr.builtin
+               (YulSemantics.EVM.Op.sub)
+               [YulSemantics.Expr.var "\x00144", YulSemantics.Expr.var "\x00154"],
+             YulSemantics.Expr.builtin
+               (YulSemantics.EVM.Op.lt)
+               [YulSemantics.Expr.var "\x00144", YulSemantics.Expr.var "\x00154"]])),
+       YulSemantics.Stmt.letDecl
+         ["\x00156"]
+         (some (YulSemantics.Expr.builtin
+            (YulSemantics.EVM.Op.add)
+            [YulSemantics.Expr.var "\x00145", YulSemantics.Expr.var "\x00146"])),
+       YulSemantics.Stmt.letDecl
+         ["\x00157"]
+         (some (YulSemantics.Expr.builtin
+            (YulSemantics.EVM.Op.lt)
+            [YulSemantics.Expr.var "\x00156", YulSemantics.Expr.var "\x00145"])),
+       YulSemantics.Stmt.assign
+         ["\x00156"]
+         (YulSemantics.Expr.builtin
+           (YulSemantics.EVM.Op.add)
+           [YulSemantics.Expr.var "\x00156", YulSemantics.Expr.var "\x00150"]),
+       YulSemantics.Stmt.assign
+         ["\x00157"]
+         (YulSemantics.Expr.builtin
+           (YulSemantics.EVM.Op.add)
+           [YulSemantics.Expr.var "\x00157",
+            YulSemantics.Expr.builtin
+              (YulSemantics.EVM.Op.lt)
+              [YulSemantics.Expr.var "\x00156", YulSemantics.Expr.var "\x00150"]]),
+       YulSemantics.Stmt.assign
+         ["\x00156"]
+         (YulSemantics.Expr.builtin
+           (YulSemantics.EVM.Op.add)
+           [YulSemantics.Expr.var "\x00147", YulSemantics.Expr.var "\x00151"]),
+       YulSemantics.Stmt.letDecl
+         ["\x00158"]
+         (some (YulSemantics.Expr.builtin
+            (YulSemantics.EVM.Op.lt)
+            [YulSemantics.Expr.var "\x00156", YulSemantics.Expr.var "\x00147"])),
+       YulSemantics.Stmt.assign
+         ["\x00156"]
+         (YulSemantics.Expr.builtin
+           (YulSemantics.EVM.Op.add)
+           [YulSemantics.Expr.var "\x00156", YulSemantics.Expr.var "\x00148"]),
+       YulSemantics.Stmt.assign
+         ["\x00158"]
+         (YulSemantics.Expr.builtin
+           (YulSemantics.EVM.Op.add)
+           [YulSemantics.Expr.var "\x00158",
+            YulSemantics.Expr.builtin
+              (YulSemantics.EVM.Op.lt)
+              [YulSemantics.Expr.var "\x00156", YulSemantics.Expr.var "\x00148"]]),
+       YulSemantics.Stmt.assign
+         ["\x00156"]
+         (YulSemantics.Expr.builtin
+           (YulSemantics.EVM.Op.add)
+           [YulSemantics.Expr.var "\x00156", YulSemantics.Expr.var "\x00152"]),
+       YulSemantics.Stmt.assign
+         ["\x00158"]
+         (YulSemantics.Expr.builtin
+           (YulSemantics.EVM.Op.add)
+           [YulSemantics.Expr.var "\x00158",
+            YulSemantics.Expr.builtin
+              (YulSemantics.EVM.Op.lt)
+              [YulSemantics.Expr.var "\x00156", YulSemantics.Expr.var "\x00152"]]),
+       YulSemantics.Stmt.assign
+         ["\x00156"]
+         (YulSemantics.Expr.builtin
+           (YulSemantics.EVM.Op.add)
+           [YulSemantics.Expr.var "\x00156", YulSemantics.Expr.var "\x00157"]),
+       YulSemantics.Stmt.assign
+         ["\x00158"]
+         (YulSemantics.Expr.builtin
+           (YulSemantics.EVM.Op.add)
+           [YulSemantics.Expr.var "\x00158",
+            YulSemantics.Expr.builtin
+              (YulSemantics.EVM.Op.lt)
+              [YulSemantics.Expr.var "\x00156", YulSemantics.Expr.var "\x00157"]]),
+       YulSemantics.Stmt.assign
+         ["\x00138"]
+         (YulSemantics.Expr.builtin
+           (YulSemantics.EVM.Op.add)
+           [YulSemantics.Expr.var "\x00149", YulSemantics.Expr.var "\x00153"]),
+       YulSemantics.Stmt.assign
+         ["\x00157"]
+         (YulSemantics.Expr.builtin
+           (YulSemantics.EVM.Op.lt)
+           [YulSemantics.Expr.var "\x00138", YulSemantics.Expr.var "\x00149"]),
+       YulSemantics.Stmt.assign
+         ["\x00138"]
+         (YulSemantics.Expr.builtin
+           (YulSemantics.EVM.Op.add)
+           [YulSemantics.Expr.var "\x00138", YulSemantics.Expr.var "\x00154"]),
+       YulSemantics.Stmt.assign
+         ["\x00157"]
+         (YulSemantics.Expr.builtin
+           (YulSemantics.EVM.Op.add)
+           [YulSemantics.Expr.var "\x00157",
+            YulSemantics.Expr.builtin
+              (YulSemantics.EVM.Op.lt)
+              [YulSemantics.Expr.var "\x00138", YulSemantics.Expr.var "\x00154"]]),
+       YulSemantics.Stmt.assign
+         ["\x00138"]
+         (YulSemantics.Expr.builtin
+           (YulSemantics.EVM.Op.add)
+           [YulSemantics.Expr.var "\x00138", YulSemantics.Expr.var "\x00158"]),
+       YulSemantics.Stmt.assign
+         ["\x00157"]
+         (YulSemantics.Expr.builtin
+           (YulSemantics.EVM.Op.add)
+           [YulSemantics.Expr.var "\x00157",
+            YulSemantics.Expr.builtin
+              (YulSemantics.EVM.Op.lt)
+              [YulSemantics.Expr.var "\x00138", YulSemantics.Expr.var "\x00158"]]),
+       YulSemantics.Stmt.assign
+         ["\x00139"]
+         (YulSemantics.Expr.builtin
+           (YulSemantics.EVM.Op.add)
+           [YulSemantics.Expr.var "\x00155", YulSemantics.Expr.var "\x00157"])],
+    YulSemantics.Stmt.letDecl
+      ["\x00159"]
+      (some (YulSemantics.Expr.lit (YulSemantics.Literal.number 34565483545414906068789196026815425751))),
+    YulSemantics.Stmt.letDecl
+      ["\x00160"]
+      (some (YulSemantics.Expr.lit
+         (YulSemantics.Literal.number 45442060874369865957053122457065728162598490762543039060009208264153100167851))),
+    YulSemantics.Stmt.block
+      [YulSemantics.Stmt.letDecl
+         ["\x00161"]
+         (some (YulSemantics.Expr.builtin
+            (YulSemantics.EVM.Op.mul)
+            [YulSemantics.Expr.var "\x00138", YulSemantics.Expr.var "\x00160"])),
+       YulSemantics.Stmt.letDecl
+         ["\x00162"]
+         (some (YulSemantics.Expr.builtin
+            (YulSemantics.EVM.Op.mulmod)
+            [YulSemantics.Expr.var "\x00138",
+             YulSemantics.Expr.var "\x00160",
+             YulSemantics.Expr.builtin
+               (YulSemantics.EVM.Op.not)
+               [YulSemantics.Expr.lit (YulSemantics.Literal.number 0)]])),
+       YulSemantics.Stmt.letDecl
+         ["\x00163"]
+         (some (YulSemantics.Expr.builtin
+            (YulSemantics.EVM.Op.sub)
+            [YulSemantics.Expr.builtin
+               (YulSemantics.EVM.Op.sub)
+               [YulSemantics.Expr.var "\x00162", YulSemantics.Expr.var "\x00161"],
+             YulSemantics.Expr.builtin
+               (YulSemantics.EVM.Op.lt)
+               [YulSemantics.Expr.var "\x00162", YulSemantics.Expr.var "\x00161"]])),
+       YulSemantics.Stmt.assign
+         ["\x00163"]
+         (YulSemantics.Expr.builtin
+           (YulSemantics.EVM.Op.add)
+           [YulSemantics.Expr.builtin
+              (YulSemantics.EVM.Op.add)
+              [YulSemantics.Expr.var "\x00163",
+               YulSemantics.Expr.builtin
+                 (YulSemantics.EVM.Op.mul)
+                 [YulSemantics.Expr.var "\x00138", YulSemantics.Expr.var "\x00159"]],
+            YulSemantics.Expr.builtin
+              (YulSemantics.EVM.Op.mul)
+              [YulSemantics.Expr.var "\x00139", YulSemantics.Expr.var "\x00160"]]),
+       YulSemantics.Stmt.assign
+         ["\x00137"]
+         (YulSemantics.Expr.builtin
+           (YulSemantics.EVM.Op.sub)
+           [YulSemantics.Expr.var "\x00135", YulSemantics.Expr.var "\x00161"]),
+       YulSemantics.Stmt.assign
+         ["\x00136"]
+         (YulSemantics.Expr.builtin
+           (YulSemantics.EVM.Op.sub)
+           [YulSemantics.Expr.builtin
+              (YulSemantics.EVM.Op.sub)
+              [YulSemantics.Expr.var "\x00134", YulSemantics.Expr.var "\x00163"],
+            YulSemantics.Expr.builtin
+              (YulSemantics.EVM.Op.lt)
+              [YulSemantics.Expr.var "\x00135", YulSemantics.Expr.var "\x00161"]])],
+    YulSemantics.Stmt.cond
+      (YulSemantics.Expr.call "\x000" [YulSemantics.Expr.var "\x00136", YulSemantics.Expr.var "\x00137"])
+      [YulSemantics.Stmt.letDecl
+         ["\x00164"]
+         (some (YulSemantics.Expr.builtin
+            (YulSemantics.EVM.Op.sub)
+            [YulSemantics.Expr.var "\x00137", YulSemantics.Expr.var "\x00160"])),
+       YulSemantics.Stmt.assign
+         ["\x00136"]
+         (YulSemantics.Expr.builtin
+           (YulSemantics.EVM.Op.sub)
+           [YulSemantics.Expr.builtin
+              (YulSemantics.EVM.Op.sub)
+              [YulSemantics.Expr.var "\x00136", YulSemantics.Expr.var "\x00159"],
+            YulSemantics.Expr.builtin
+              (YulSemantics.EVM.Op.gt)
+              [YulSemantics.Expr.var "\x00160", YulSemantics.Expr.var "\x00137"]]),
+       YulSemantics.Stmt.assign ["\x00137"] (YulSemantics.Expr.var "\x00164")],
+    YulSemantics.Stmt.cond
+      (YulSemantics.Expr.call "\x000" [YulSemantics.Expr.var "\x00136", YulSemantics.Expr.var "\x00137"])
+      [YulSemantics.Stmt.letDecl
+         ["\x00165"]
+         (some (YulSemantics.Expr.builtin
+            (YulSemantics.EVM.Op.sub)
+            [YulSemantics.Expr.var "\x00137", YulSemantics.Expr.var "\x00160"])),
+       YulSemantics.Stmt.assign
+         ["\x00136"]
+         (YulSemantics.Expr.builtin
+           (YulSemantics.EVM.Op.sub)
+           [YulSemantics.Expr.builtin
+              (YulSemantics.EVM.Op.sub)
+              [YulSemantics.Expr.var "\x00136", YulSemantics.Expr.var "\x00159"],
+            YulSemantics.Expr.builtin
+              (YulSemantics.EVM.Op.gt)
+              [YulSemantics.Expr.var "\x00160", YulSemantics.Expr.var "\x00137"]]),
+       YulSemantics.Stmt.assign ["\x00137"] (YulSemantics.Expr.var "\x00165")]],
+ YulSemantics.Stmt.funDef
+   "\x0015"
+   ["\x00166", "\x00167", "\x00168", "\x00169"]
+   ["\x00170", "\x00171"]
+   [YulSemantics.Stmt.letDecl ["\x00172"] (some (YulSemantics.Expr.lit (YulSemantics.Literal.number 0))),
+    YulSemantics.Stmt.letDecl ["\x00173"] (some (YulSemantics.Expr.lit (YulSemantics.Literal.number 0))),
+    YulSemantics.Stmt.letDecl ["\x00174"] (some (YulSemantics.Expr.lit (YulSemantics.Literal.number 0))),
+    YulSemantics.Stmt.block
+      [YulSemantics.Stmt.letDecl
+         ["\x00175"]
+         (some (YulSemantics.Expr.builtin
+            (YulSemantics.EVM.Op.mul)
+            [YulSemantics.Expr.var "\x00166", YulSemantics.Expr.var "\x00168"])),
+       YulSemantics.Stmt.letDecl
+         ["\x00176"]
+         (some (YulSemantics.Expr.builtin
+            (YulSemantics.EVM.Op.mulmod)
+            [YulSemantics.Expr.var "\x00166",
+             YulSemantics.Expr.var "\x00168",
+             YulSemantics.Expr.builtin
+               (YulSemantics.EVM.Op.not)
+               [YulSemantics.Expr.lit (YulSemantics.Literal.number 0)]])),
+       YulSemantics.Stmt.letDecl
+         ["\x00177"]
+         (some (YulSemantics.Expr.builtin
+            (YulSemantics.EVM.Op.sub)
+            [YulSemantics.Expr.builtin
+               (YulSemantics.EVM.Op.sub)
+               [YulSemantics.Expr.var "\x00176", YulSemantics.Expr.var "\x00175"],
+             YulSemantics.Expr.builtin
+               (YulSemantics.EVM.Op.lt)
+               [YulSemantics.Expr.var "\x00176", YulSemantics.Expr.var "\x00175"]])),
+       YulSemantics.Stmt.assign ["\x00172"] (YulSemantics.Expr.var "\x00175"),
+       YulSemantics.Stmt.letDecl ["\x00178"] (some (YulSemantics.Expr.var "\x00177")),
+       YulSemantics.Stmt.assign
+         ["\x00175"]
+         (YulSemantics.Expr.builtin
+           (YulSemantics.EVM.Op.mul)
+           [YulSemantics.Expr.var "\x00166", YulSemantics.Expr.var "\x00169"]),
+       YulSemantics.Stmt.assign
+         ["\x00176"]
+         (YulSemantics.Expr.builtin
+           (YulSemantics.EVM.Op.mulmod)
+           [YulSemantics.Expr.var "\x00166",
+            YulSemantics.Expr.var "\x00169",
+            YulSemantics.Expr.builtin
+              (YulSemantics.EVM.Op.not)
+              [YulSemantics.Expr.lit (YulSemantics.Literal.number 0)]]),
+       YulSemantics.Stmt.assign
+         ["\x00177"]
+         (YulSemantics.Expr.builtin
+           (YulSemantics.EVM.Op.sub)
+           [YulSemantics.Expr.builtin
+              (YulSemantics.EVM.Op.sub)
+              [YulSemantics.Expr.var "\x00176", YulSemantics.Expr.var "\x00175"],
+            YulSemantics.Expr.builtin
+              (YulSemantics.EVM.Op.lt)
+              [YulSemantics.Expr.var "\x00176", YulSemantics.Expr.var "\x00175"]]),
+       YulSemantics.Stmt.letDecl
+         ["\x00179"]
+         (some (YulSemantics.Expr.builtin
+            (YulSemantics.EVM.Op.add)
+            [YulSemantics.Expr.var "\x00175", YulSemantics.Expr.var "\x00178"])),
+       YulSemantics.Stmt.assign ["\x00173"] (YulSemantics.Expr.var "\x00179"),
+       YulSemantics.Stmt.assign
+         ["\x00174"]
+         (YulSemantics.Expr.builtin
+           (YulSemantics.EVM.Op.add)
+           [YulSemantics.Expr.var "\x00177",
+            YulSemantics.Expr.builtin
+              (YulSemantics.EVM.Op.lt)
+              [YulSemantics.Expr.var "\x00179", YulSemantics.Expr.var "\x00175"]])],
+    YulSemantics.Stmt.letDecl
+      ["\x00180"]
+      (some (YulSemantics.Expr.builtin
+         (YulSemantics.EVM.Op.mul)
+         [YulSemantics.Expr.var "\x00172",
+          YulSemantics.Expr.lit
+            (YulSemantics.Literal.number
+              11726191667098586211898467594267748916577995138249226639719947807923487178749)])),
+    YulSemantics.Stmt.block
+      [YulSemantics.Stmt.letDecl
+         ["\x00181"]
+         (some (YulSemantics.Expr.lit
+            (YulSemantics.Literal.number
+              45442060874369865957053122457065728162598490762543039060009208264153100167851))),
+       YulSemantics.Stmt.letDecl
+         ["\x00182"]
+         (some (YulSemantics.Expr.builtin
+            (YulSemantics.EVM.Op.mul)
+            [YulSemantics.Expr.var "\x00180", YulSemantics.Expr.var "\x00181"])),
+       YulSemantics.Stmt.letDecl
+         ["\x00183"]
+         (some (YulSemantics.Expr.builtin
+            (YulSemantics.EVM.Op.mulmod)
+            [YulSemantics.Expr.var "\x00180",
+             YulSemantics.Expr.var "\x00181",
+             YulSemantics.Expr.builtin
+               (YulSemantics.EVM.Op.not)
+               [YulSemantics.Expr.lit (YulSemantics.Literal.number 0)]])),
+       YulSemantics.Stmt.letDecl
+         ["\x00184"]
+         (some (YulSemantics.Expr.builtin
+            (YulSemantics.EVM.Op.sub)
+            [YulSemantics.Expr.builtin
+               (YulSemantics.EVM.Op.sub)
+               [YulSemantics.Expr.var "\x00183", YulSemantics.Expr.var "\x00182"],
+             YulSemantics.Expr.builtin
+               (YulSemantics.EVM.Op.lt)
+               [YulSemantics.Expr.var "\x00183", YulSemantics.Expr.var "\x00182"]])),
+       YulSemantics.Stmt.letDecl
+         ["\x00185"]
+         (some (YulSemantics.Expr.builtin
+            (YulSemantics.EVM.Op.add)
+            [YulSemantics.Expr.var "\x00172", YulSemantics.Expr.var "\x00182"])),
+       YulSemantics.Stmt.letDecl
+         ["\x00186"]
+         (some (YulSemantics.Expr.builtin
+            (YulSemantics.EVM.Op.add)
+            [YulSemantics.Expr.var "\x00184",
+             YulSemantics.Expr.builtin
+               (YulSemantics.EVM.Op.lt)
+               [YulSemantics.Expr.var "\x00185", YulSemantics.Expr.var "\x00172"]])),
+       YulSemantics.Stmt.letDecl
+         ["\x00187"]
+         (some (YulSemantics.Expr.lit (YulSemantics.Literal.number 34565483545414906068789196026815425751))),
+       YulSemantics.Stmt.assign
+         ["\x00182"]
+         (YulSemantics.Expr.builtin
+           (YulSemantics.EVM.Op.mul)
+           [YulSemantics.Expr.var "\x00180", YulSemantics.Expr.var "\x00187"]),
+       YulSemantics.Stmt.assign
+         ["\x00183"]
+         (YulSemantics.Expr.builtin
+           (YulSemantics.EVM.Op.mulmod)
+           [YulSemantics.Expr.var "\x00180",
+            YulSemantics.Expr.var "\x00187",
+            YulSemantics.Expr.builtin
+              (YulSemantics.EVM.Op.not)
+              [YulSemantics.Expr.lit (YulSemantics.Literal.number 0)]]),
+       YulSemantics.Stmt.assign
+         ["\x00184"]
+         (YulSemantics.Expr.builtin
+           (YulSemantics.EVM.Op.sub)
+           [YulSemantics.Expr.builtin
+              (YulSemantics.EVM.Op.sub)
+              [YulSemantics.Expr.var "\x00183", YulSemantics.Expr.var "\x00182"],
+            YulSemantics.Expr.builtin
+              (YulSemantics.EVM.Op.lt)
+              [YulSemantics.Expr.var "\x00183", YulSemantics.Expr.var "\x00182"]]),
+       YulSemantics.Stmt.assign
+         ["\x00185"]
+         (YulSemantics.Expr.builtin
+           (YulSemantics.EVM.Op.add)
+           [YulSemantics.Expr.var "\x00173", YulSemantics.Expr.var "\x00182"]),
+       YulSemantics.Stmt.letDecl
+         ["\x00188"]
+         (some (YulSemantics.Expr.builtin
+            (YulSemantics.EVM.Op.lt)
+            [YulSemantics.Expr.var "\x00185", YulSemantics.Expr.var "\x00173"])),
+       YulSemantics.Stmt.letDecl
+         ["\x00189"]
+         (some (YulSemantics.Expr.builtin
+            (YulSemantics.EVM.Op.add)
+            [YulSemantics.Expr.var "\x00185", YulSemantics.Expr.var "\x00186"])),
+       YulSemantics.Stmt.letDecl
+         ["\x00190"]
+         (some (YulSemantics.Expr.builtin
+            (YulSemantics.EVM.Op.lt)
+            [YulSemantics.Expr.var "\x00189", YulSemantics.Expr.var "\x00185"])),
+       YulSemantics.Stmt.assign ["\x00172"] (YulSemantics.Expr.var "\x00189"),
+       YulSemantics.Stmt.assign
+         ["\x00173"]
+         (YulSemantics.Expr.builtin
+           (YulSemantics.EVM.Op.add)
+           [YulSemantics.Expr.var "\x00174",
+            YulSemantics.Expr.builtin
+              (YulSemantics.EVM.Op.add)
+              [YulSemantics.Expr.var "\x00184",
+               YulSemantics.Expr.builtin
+                 (YulSemantics.EVM.Op.add)
+                 [YulSemantics.Expr.var "\x00188", YulSemantics.Expr.var "\x00190"]]]),
+       YulSemantics.Stmt.assign ["\x00174"] (YulSemantics.Expr.lit (YulSemantics.Literal.number 0))],
+    YulSemantics.Stmt.block
+      [YulSemantics.Stmt.letDecl
+         ["\x00191"]
+         (some (YulSemantics.Expr.builtin
+            (YulSemantics.EVM.Op.mul)
+            [YulSemantics.Expr.var "\x00167", YulSemantics.Expr.var "\x00168"])),
+       YulSemantics.Stmt.letDecl
+         ["\x00192"]
+         (some (YulSemantics.Expr.builtin
+            (YulSemantics.EVM.Op.mulmod)
+            [YulSemantics.Expr.var "\x00167",
+             YulSemantics.Expr.var "\x00168",
+             YulSemantics.Expr.builtin
+               (YulSemantics.EVM.Op.not)
+               [YulSemantics.Expr.lit (YulSemantics.Literal.number 0)]])),
+       YulSemantics.Stmt.letDecl
+         ["\x00193"]
+         (some (YulSemantics.Expr.builtin
+            (YulSemantics.EVM.Op.sub)
+            [YulSemantics.Expr.builtin
+               (YulSemantics.EVM.Op.sub)
+               [YulSemantics.Expr.var "\x00192", YulSemantics.Expr.var "\x00191"],
+             YulSemantics.Expr.builtin
+               (YulSemantics.EVM.Op.lt)
+               [YulSemantics.Expr.var "\x00192", YulSemantics.Expr.var "\x00191"]])),
+       YulSemantics.Stmt.letDecl
+         ["\x00194"]
+         (some (YulSemantics.Expr.builtin
+            (YulSemantics.EVM.Op.add)
+            [YulSemantics.Expr.var "\x00172", YulSemantics.Expr.var "\x00191"])),
+       YulSemantics.Stmt.letDecl
+         ["\x00195"]
+         (some (YulSemantics.Expr.builtin
+            (YulSemantics.EVM.Op.add)
+            [YulSemantics.Expr.var "\x00193",
+             YulSemantics.Expr.builtin
+               (YulSemantics.EVM.Op.lt)
+               [YulSemantics.Expr.var "\x00194", YulSemantics.Expr.var "\x00172"]])),
+       YulSemantics.Stmt.assign ["\x00172"] (YulSemantics.Expr.var "\x00194"),
+       YulSemantics.Stmt.assign
+         ["\x00191"]
+         (YulSemantics.Expr.builtin
+           (YulSemantics.EVM.Op.mul)
+           [YulSemantics.Expr.var "\x00167", YulSemantics.Expr.var "\x00169"]),
+       YulSemantics.Stmt.assign
+         ["\x00192"]
+         (YulSemantics.Expr.builtin
+           (YulSemantics.EVM.Op.mulmod)
+           [YulSemantics.Expr.var "\x00167",
+            YulSemantics.Expr.var "\x00169",
+            YulSemantics.Expr.builtin
+              (YulSemantics.EVM.Op.not)
+              [YulSemantics.Expr.lit (YulSemantics.Literal.number 0)]]),
+       YulSemantics.Stmt.assign
+         ["\x00193"]
+         (YulSemantics.Expr.builtin
+           (YulSemantics.EVM.Op.sub)
+           [YulSemantics.Expr.builtin
+              (YulSemantics.EVM.Op.sub)
+              [YulSemantics.Expr.var "\x00192", YulSemantics.Expr.var "\x00191"],
+            YulSemantics.Expr.builtin
+              (YulSemantics.EVM.Op.lt)
+              [YulSemantics.Expr.var "\x00192", YulSemantics.Expr.var "\x00191"]]),
+       YulSemantics.Stmt.assign
+         ["\x00194"]
+         (YulSemantics.Expr.builtin
+           (YulSemantics.EVM.Op.add)
+           [YulSemantics.Expr.var "\x00173", YulSemantics.Expr.var "\x00191"]),
+       YulSemantics.Stmt.letDecl
+         ["\x00196"]
+         (some (YulSemantics.Expr.builtin
+            (YulSemantics.EVM.Op.lt)
+            [YulSemantics.Expr.var "\x00194", YulSemantics.Expr.var "\x00173"])),
+       YulSemantics.Stmt.letDecl
+         ["\x00197"]
+         (some (YulSemantics.Expr.builtin
+            (YulSemantics.EVM.Op.add)
+            [YulSemantics.Expr.var "\x00194", YulSemantics.Expr.var "\x00195"])),
+       YulSemantics.Stmt.letDecl
+         ["\x00198"]
+         (some (YulSemantics.Expr.builtin
+            (YulSemantics.EVM.Op.lt)
+            [YulSemantics.Expr.var "\x00197", YulSemantics.Expr.var "\x00194"])),
+       YulSemantics.Stmt.assign ["\x00173"] (YulSemantics.Expr.var "\x00197"),
+       YulSemantics.Stmt.assign
+         ["\x00174"]
+         (YulSemantics.Expr.builtin
+           (YulSemantics.EVM.Op.add)
+           [YulSemantics.Expr.var "\x00193",
+            YulSemantics.Expr.builtin
+              (YulSemantics.EVM.Op.add)
+              [YulSemantics.Expr.var "\x00196", YulSemantics.Expr.var "\x00198"]])],
+    YulSemantics.Stmt.assign
+      ["\x00180"]
+      (YulSemantics.Expr.builtin
+        (YulSemantics.EVM.Op.mul)
+        [YulSemantics.Expr.var "\x00172",
+         YulSemantics.Expr.lit
+           (YulSemantics.Literal.number
+             11726191667098586211898467594267748916577995138249226639719947807923487178749)]),
+    YulSemantics.Stmt.block
+      [YulSemantics.Stmt.letDecl
+         ["\x00199"]
+         (some (YulSemantics.Expr.lit
+            (YulSemantics.Literal.number
+              45442060874369865957053122457065728162598490762543039060009208264153100167851))),
+       YulSemantics.Stmt.letDecl
+         ["\x00200"]
+         (some (YulSemantics.Expr.builtin
+            (YulSemantics.EVM.Op.mul)
+            [YulSemantics.Expr.var "\x00180", YulSemantics.Expr.var "\x00199"])),
+       YulSemantics.Stmt.letDecl
+         ["\x00201"]
+         (some (YulSemantics.Expr.builtin
+            (YulSemantics.EVM.Op.mulmod)
+            [YulSemantics.Expr.var "\x00180",
+             YulSemantics.Expr.var "\x00199",
+             YulSemantics.Expr.builtin
+               (YulSemantics.EVM.Op.not)
+               [YulSemantics.Expr.lit (YulSemantics.Literal.number 0)]])),
+       YulSemantics.Stmt.letDecl
+         ["\x00202"]
+         (some (YulSemantics.Expr.builtin
+            (YulSemantics.EVM.Op.sub)
+            [YulSemantics.Expr.builtin
+               (YulSemantics.EVM.Op.sub)
+               [YulSemantics.Expr.var "\x00201", YulSemantics.Expr.var "\x00200"],
+             YulSemantics.Expr.builtin
+               (YulSemantics.EVM.Op.lt)
+               [YulSemantics.Expr.var "\x00201", YulSemantics.Expr.var "\x00200"]])),
+       YulSemantics.Stmt.letDecl
+         ["\x00203"]
+         (some (YulSemantics.Expr.builtin
+            (YulSemantics.EVM.Op.add)
+            [YulSemantics.Expr.var "\x00172", YulSemantics.Expr.var "\x00200"])),
+       YulSemantics.Stmt.letDecl
+         ["\x00204"]
+         (some (YulSemantics.Expr.builtin
+            (YulSemantics.EVM.Op.add)
+            [YulSemantics.Expr.var "\x00202",
+             YulSemantics.Expr.builtin
+               (YulSemantics.EVM.Op.lt)
+               [YulSemantics.Expr.var "\x00203", YulSemantics.Expr.var "\x00172"]])),
+       YulSemantics.Stmt.letDecl
+         ["\x00205"]
+         (some (YulSemantics.Expr.lit (YulSemantics.Literal.number 34565483545414906068789196026815425751))),
+       YulSemantics.Stmt.assign
+         ["\x00200"]
+         (YulSemantics.Expr.builtin
+           (YulSemantics.EVM.Op.mul)
+           [YulSemantics.Expr.var "\x00180", YulSemantics.Expr.var "\x00205"]),
+       YulSemantics.Stmt.assign
+         ["\x00201"]
+         (YulSemantics.Expr.builtin
+           (YulSemantics.EVM.Op.mulmod)
+           [YulSemantics.Expr.var "\x00180",
+            YulSemantics.Expr.var "\x00205",
+            YulSemantics.Expr.builtin
+              (YulSemantics.EVM.Op.not)
+              [YulSemantics.Expr.lit (YulSemantics.Literal.number 0)]]),
+       YulSemantics.Stmt.assign
+         ["\x00202"]
+         (YulSemantics.Expr.builtin
+           (YulSemantics.EVM.Op.sub)
+           [YulSemantics.Expr.builtin
+              (YulSemantics.EVM.Op.sub)
+              [YulSemantics.Expr.var "\x00201", YulSemantics.Expr.var "\x00200"],
+            YulSemantics.Expr.builtin
+              (YulSemantics.EVM.Op.lt)
+              [YulSemantics.Expr.var "\x00201", YulSemantics.Expr.var "\x00200"]]),
+       YulSemantics.Stmt.assign
+         ["\x00203"]
+         (YulSemantics.Expr.builtin
+           (YulSemantics.EVM.Op.add)
+           [YulSemantics.Expr.var "\x00173", YulSemantics.Expr.var "\x00200"]),
+       YulSemantics.Stmt.letDecl
+         ["\x00206"]
+         (some (YulSemantics.Expr.builtin
+            (YulSemantics.EVM.Op.lt)
+            [YulSemantics.Expr.var "\x00203", YulSemantics.Expr.var "\x00173"])),
+       YulSemantics.Stmt.letDecl
+         ["\x00207"]
+         (some (YulSemantics.Expr.builtin
+            (YulSemantics.EVM.Op.add)
+            [YulSemantics.Expr.var "\x00203", YulSemantics.Expr.var "\x00204"])),
+       YulSemantics.Stmt.letDecl
+         ["\x00208"]
+         (some (YulSemantics.Expr.builtin
+            (YulSemantics.EVM.Op.lt)
+            [YulSemantics.Expr.var "\x00207", YulSemantics.Expr.var "\x00203"])),
+       YulSemantics.Stmt.assign ["\x00170"] (YulSemantics.Expr.var "\x00207"),
+       YulSemantics.Stmt.assign
+         ["\x00171"]
+         (YulSemantics.Expr.builtin
+           (YulSemantics.EVM.Op.add)
+           [YulSemantics.Expr.var "\x00174",
+            YulSemantics.Expr.builtin
+              (YulSemantics.EVM.Op.add)
+              [YulSemantics.Expr.var "\x00202",
+               YulSemantics.Expr.builtin
+                 (YulSemantics.EVM.Op.add)
+                 [YulSemantics.Expr.var "\x00206", YulSemantics.Expr.var "\x00208"]]])],
+    YulSemantics.Stmt.cond
+      (YulSemantics.Expr.call "\x000" [YulSemantics.Expr.var "\x00171", YulSemantics.Expr.var "\x00170"])
+      [YulSemantics.Stmt.letDecl
+         ["\x00209"]
+         (some (YulSemantics.Expr.lit (YulSemantics.Literal.number 34565483545414906068789196026815425751))),
+       YulSemantics.Stmt.letDecl
+         ["\x00210"]
+         (some (YulSemantics.Expr.lit
+            (YulSemantics.Literal.number
+              45442060874369865957053122457065728162598490762543039060009208264153100167851))),
+       YulSemantics.Stmt.letDecl
+         ["\x00211"]
+         (some (YulSemantics.Expr.builtin
+            (YulSemantics.EVM.Op.sub)
+            [YulSemantics.Expr.var "\x00170", YulSemantics.Expr.var "\x00210"])),
+       YulSemantics.Stmt.assign
+         ["\x00171"]
+         (YulSemantics.Expr.builtin
+           (YulSemantics.EVM.Op.sub)
+           [YulSemantics.Expr.builtin
+              (YulSemantics.EVM.Op.sub)
+              [YulSemantics.Expr.var "\x00171", YulSemantics.Expr.var "\x00209"],
+            YulSemantics.Expr.builtin
+              (YulSemantics.EVM.Op.gt)
+              [YulSemantics.Expr.var "\x00210", YulSemantics.Expr.var "\x00170"]]),
+       YulSemantics.Stmt.assign ["\x00170"] (YulSemantics.Expr.var "\x00211")]],
  YulSemantics.Stmt.cond
    (YulSemantics.Expr.builtin
      (YulSemantics.EVM.Op.iszero)
@@ -646,7 +1418,7 @@ def frozenReferenceBlock : Block Op :=
    [YulSemantics.Stmt.exprStmt (YulSemantics.Expr.builtin (YulSemantics.EVM.Op.invalid) [])],
  YulSemantics.Stmt.block
    [YulSemantics.Stmt.letDecl
-      ["\x0096"]
+      ["\x0099"]
       (some (YulSemantics.Expr.builtin
          (YulSemantics.EVM.Op.and)
          [YulSemantics.Expr.call
@@ -666,7 +1438,7 @@ def frozenReferenceBlock : Block Op :=
                (YulSemantics.EVM.Op.mload)
                [YulSemantics.Expr.lit (YulSemantics.Literal.number 96)]]])),
     YulSemantics.Stmt.letDecl
-      ["\x0097"]
+      ["\x00100"]
       (some (YulSemantics.Expr.builtin
          (YulSemantics.EVM.Op.and)
          [YulSemantics.Expr.call
@@ -688,7 +1460,7 @@ def frozenReferenceBlock : Block Op :=
     YulSemantics.Stmt.cond
       (YulSemantics.Expr.builtin
         (YulSemantics.EVM.Op.and)
-        [YulSemantics.Expr.builtin (YulSemantics.EVM.Op.iszero) [YulSemantics.Expr.var "\x0096"],
+        [YulSemantics.Expr.builtin (YulSemantics.EVM.Op.iszero) [YulSemantics.Expr.var "\x0099"],
          YulSemantics.Expr.builtin
            (YulSemantics.EVM.Op.iszero)
            [YulSemantics.Expr.call
@@ -709,7 +1481,7 @@ def frozenReferenceBlock : Block Op :=
     YulSemantics.Stmt.cond
       (YulSemantics.Expr.builtin
         (YulSemantics.EVM.Op.and)
-        [YulSemantics.Expr.builtin (YulSemantics.EVM.Op.iszero) [YulSemantics.Expr.var "\x0097"],
+        [YulSemantics.Expr.builtin (YulSemantics.EVM.Op.iszero) [YulSemantics.Expr.var "\x00100"],
          YulSemantics.Expr.builtin
            (YulSemantics.EVM.Op.iszero)
            [YulSemantics.Expr.call
@@ -730,14 +1502,14 @@ def frozenReferenceBlock : Block Op :=
     YulSemantics.Stmt.cond
       (YulSemantics.Expr.builtin
         (YulSemantics.EVM.Op.and)
-        [YulSemantics.Expr.var "\x0096", YulSemantics.Expr.var "\x0097"])
+        [YulSemantics.Expr.var "\x0099", YulSemantics.Expr.var "\x00100"])
       [YulSemantics.Stmt.exprStmt
          (YulSemantics.Expr.builtin
            (YulSemantics.EVM.Op.ret)
            [YulSemantics.Expr.lit (YulSemantics.Literal.number 0),
             YulSemantics.Expr.lit (YulSemantics.Literal.number 128)])],
     YulSemantics.Stmt.cond
-      (YulSemantics.Expr.var "\x0096")
+      (YulSemantics.Expr.var "\x0099")
       [YulSemantics.Stmt.exprStmt
          (YulSemantics.Expr.call
            "\x0012"
@@ -759,13 +1531,13 @@ def frozenReferenceBlock : Block Op :=
            [YulSemantics.Expr.lit (YulSemantics.Literal.number 0),
             YulSemantics.Expr.lit (YulSemantics.Literal.number 128)])],
     YulSemantics.Stmt.cond
-      (YulSemantics.Expr.var "\x0097")
+      (YulSemantics.Expr.var "\x00100")
       [YulSemantics.Stmt.exprStmt
          (YulSemantics.Expr.builtin
            (YulSemantics.EVM.Op.ret)
            [YulSemantics.Expr.lit (YulSemantics.Literal.number 0),
             YulSemantics.Expr.lit (YulSemantics.Literal.number 128)])]],
- YulSemantics.Stmt.letDecl ["\x0098", "\x0099"] none,
+ YulSemantics.Stmt.letDecl ["\x00101", "\x00102"] none,
  YulSemantics.Stmt.cond
    (YulSemantics.Expr.call
      "\x003"
@@ -822,7 +1594,7 @@ def frozenReferenceBlock : Block Op :=
            [YulSemantics.Expr.lit (YulSemantics.Literal.number 0),
             YulSemantics.Expr.lit (YulSemantics.Literal.number 128)])],
     YulSemantics.Stmt.letDecl
-      ["\x00100", "\x00101"]
+      ["\x00103", "\x00104"]
       (some (YulSemantics.Expr.call
          "\x009"
          [YulSemantics.Expr.builtin (YulSemantics.EVM.Op.mload) [YulSemantics.Expr.lit (YulSemantics.Literal.number 0)],
@@ -834,23 +1606,23 @@ def frozenReferenceBlock : Block Op :=
             (YulSemantics.EVM.Op.mload)
             [YulSemantics.Expr.lit (YulSemantics.Literal.number 32)]])),
     YulSemantics.Stmt.letDecl
-      ["\x00102", "\x00103"]
+      ["\x00105", "\x00106"]
       (some (YulSemantics.Expr.call
          "\x004"
-         [YulSemantics.Expr.var "\x00100",
-          YulSemantics.Expr.var "\x00101",
-          YulSemantics.Expr.var "\x00100",
-          YulSemantics.Expr.var "\x00101"])),
+         [YulSemantics.Expr.var "\x00103",
+          YulSemantics.Expr.var "\x00104",
+          YulSemantics.Expr.var "\x00103",
+          YulSemantics.Expr.var "\x00104"])),
     YulSemantics.Stmt.assign
-      ["\x00102", "\x00103"]
+      ["\x00105", "\x00106"]
       (YulSemantics.Expr.call
         "\x004"
-        [YulSemantics.Expr.var "\x00102",
+        [YulSemantics.Expr.var "\x00105",
+         YulSemantics.Expr.var "\x00106",
          YulSemantics.Expr.var "\x00103",
-         YulSemantics.Expr.var "\x00100",
-         YulSemantics.Expr.var "\x00101"]),
+         YulSemantics.Expr.var "\x00104"]),
     YulSemantics.Stmt.letDecl
-      ["\x00104", "\x00105"]
+      ["\x00107", "\x00108"]
       (some (YulSemantics.Expr.call
          "\x004"
          [YulSemantics.Expr.builtin
@@ -866,16 +1638,16 @@ def frozenReferenceBlock : Block Op :=
             (YulSemantics.EVM.Op.mload)
             [YulSemantics.Expr.lit (YulSemantics.Literal.number 96)]])),
     YulSemantics.Stmt.letDecl
-      ["\x00106", "\x00107"]
-      (some (YulSemantics.Expr.call "\x0010" [YulSemantics.Expr.var "\x00104", YulSemantics.Expr.var "\x00105"])),
+      ["\x00109", "\x00110"]
+      (some (YulSemantics.Expr.call "\x0010" [YulSemantics.Expr.var "\x00107", YulSemantics.Expr.var "\x00108"])),
     YulSemantics.Stmt.assign
-      ["\x0098", "\x0099"]
+      ["\x00101", "\x00102"]
       (YulSemantics.Expr.call
         "\x009"
-        [YulSemantics.Expr.var "\x00102",
-         YulSemantics.Expr.var "\x00103",
+        [YulSemantics.Expr.var "\x00105",
          YulSemantics.Expr.var "\x00106",
-         YulSemantics.Expr.var "\x00107"])],
+         YulSemantics.Expr.var "\x00109",
+         YulSemantics.Expr.var "\x00110"])],
  YulSemantics.Stmt.cond
    (YulSemantics.Expr.builtin
      (YulSemantics.EVM.Op.iszero)
@@ -890,7 +1662,7 @@ def frozenReferenceBlock : Block Op :=
            (YulSemantics.EVM.Op.mload)
            [YulSemantics.Expr.lit (YulSemantics.Literal.number 160)]]])
    [YulSemantics.Stmt.letDecl
-      ["\x00108", "\x00109"]
+      ["\x00111", "\x00112"]
       (some (YulSemantics.Expr.call
          "\x005"
          [YulSemantics.Expr.builtin
@@ -906,7 +1678,7 @@ def frozenReferenceBlock : Block Op :=
             (YulSemantics.EVM.Op.mload)
             [YulSemantics.Expr.lit (YulSemantics.Literal.number 96)]])),
     YulSemantics.Stmt.letDecl
-      ["\x00110", "\x00111"]
+      ["\x00113", "\x00114"]
       (some (YulSemantics.Expr.call
          "\x005"
          [YulSemantics.Expr.builtin
@@ -920,71 +1692,71 @@ def frozenReferenceBlock : Block Op :=
             (YulSemantics.EVM.Op.mload)
             [YulSemantics.Expr.lit (YulSemantics.Literal.number 32)]])),
     YulSemantics.Stmt.letDecl
-      ["\x00112", "\x00113"]
-      (some (YulSemantics.Expr.call "\x0010" [YulSemantics.Expr.var "\x00110", YulSemantics.Expr.var "\x00111"])),
+      ["\x00115", "\x00116"]
+      (some (YulSemantics.Expr.call "\x0010" [YulSemantics.Expr.var "\x00113", YulSemantics.Expr.var "\x00114"])),
     YulSemantics.Stmt.assign
-      ["\x0098", "\x0099"]
+      ["\x00101", "\x00102"]
       (YulSemantics.Expr.call
         "\x009"
-        [YulSemantics.Expr.var "\x00108",
-         YulSemantics.Expr.var "\x00109",
+        [YulSemantics.Expr.var "\x00111",
          YulSemantics.Expr.var "\x00112",
-         YulSemantics.Expr.var "\x00113"])],
+         YulSemantics.Expr.var "\x00115",
+         YulSemantics.Expr.var "\x00116"])],
  YulSemantics.Stmt.letDecl
-   ["\x00114", "\x00115"]
+   ["\x00117", "\x00118"]
    (some (YulSemantics.Expr.call
       "\x009"
-      [YulSemantics.Expr.var "\x0098",
-       YulSemantics.Expr.var "\x0099",
-       YulSemantics.Expr.var "\x0098",
-       YulSemantics.Expr.var "\x0099"])),
+      [YulSemantics.Expr.var "\x00101",
+       YulSemantics.Expr.var "\x00102",
+       YulSemantics.Expr.var "\x00101",
+       YulSemantics.Expr.var "\x00102"])),
  YulSemantics.Stmt.assign
-   ["\x00114", "\x00115"]
+   ["\x00117", "\x00118"]
    (YulSemantics.Expr.call
      "\x005"
-     [YulSemantics.Expr.var "\x00114",
-      YulSemantics.Expr.var "\x00115",
+     [YulSemantics.Expr.var "\x00117",
+      YulSemantics.Expr.var "\x00118",
       YulSemantics.Expr.builtin (YulSemantics.EVM.Op.mload) [YulSemantics.Expr.lit (YulSemantics.Literal.number 0)],
       YulSemantics.Expr.builtin (YulSemantics.EVM.Op.mload) [YulSemantics.Expr.lit (YulSemantics.Literal.number 32)]]),
  YulSemantics.Stmt.assign
-   ["\x00114", "\x00115"]
+   ["\x00117", "\x00118"]
    (YulSemantics.Expr.call
      "\x005"
-     [YulSemantics.Expr.var "\x00114",
-      YulSemantics.Expr.var "\x00115",
+     [YulSemantics.Expr.var "\x00117",
+      YulSemantics.Expr.var "\x00118",
       YulSemantics.Expr.builtin (YulSemantics.EVM.Op.mload) [YulSemantics.Expr.lit (YulSemantics.Literal.number 128)],
       YulSemantics.Expr.builtin (YulSemantics.EVM.Op.mload) [YulSemantics.Expr.lit (YulSemantics.Literal.number 160)]]),
  YulSemantics.Stmt.letDecl
-   ["\x00116", "\x00117"]
+   ["\x00119", "\x00120"]
    (some (YulSemantics.Expr.call
       "\x005"
       [YulSemantics.Expr.builtin (YulSemantics.EVM.Op.mload) [YulSemantics.Expr.lit (YulSemantics.Literal.number 0)],
        YulSemantics.Expr.builtin (YulSemantics.EVM.Op.mload) [YulSemantics.Expr.lit (YulSemantics.Literal.number 32)],
-       YulSemantics.Expr.var "\x00114",
-       YulSemantics.Expr.var "\x00115"])),
+       YulSemantics.Expr.var "\x00117",
+       YulSemantics.Expr.var "\x00118"])),
  YulSemantics.Stmt.letDecl
-   ["\x00118", "\x00119"]
+   ["\x00121", "\x00122"]
    (some (YulSemantics.Expr.call
       "\x009"
-      [YulSemantics.Expr.var "\x0098",
-       YulSemantics.Expr.var "\x0099",
-       YulSemantics.Expr.var "\x00116",
-       YulSemantics.Expr.var "\x00117"])),
+      [YulSemantics.Expr.var "\x00101",
+       YulSemantics.Expr.var "\x00102",
+       YulSemantics.Expr.var "\x00119",
+       YulSemantics.Expr.var "\x00120"])),
  YulSemantics.Stmt.assign
-   ["\x00118", "\x00119"]
+   ["\x00121", "\x00122"]
    (YulSemantics.Expr.call
      "\x005"
-     [YulSemantics.Expr.var "\x00118",
-      YulSemantics.Expr.var "\x00119",
+     [YulSemantics.Expr.var "\x00121",
+      YulSemantics.Expr.var "\x00122",
       YulSemantics.Expr.builtin (YulSemantics.EVM.Op.mload) [YulSemantics.Expr.lit (YulSemantics.Literal.number 64)],
       YulSemantics.Expr.builtin (YulSemantics.EVM.Op.mload) [YulSemantics.Expr.lit (YulSemantics.Literal.number 96)]]),
  YulSemantics.Stmt.exprStmt
    (YulSemantics.Expr.call
      "\x0012"
-     [YulSemantics.Expr.var "\x00114",
-      YulSemantics.Expr.var "\x00115",
+     [YulSemantics.Expr.var "\x00117",
       YulSemantics.Expr.var "\x00118",
-      YulSemantics.Expr.var "\x00119"]),
+      YulSemantics.Expr.var "\x00121",
+      YulSemantics.Expr.var "\x00122"]),
  YulSemantics.Stmt.exprStmt
    (YulSemantics.Expr.builtin
      (YulSemantics.EVM.Op.ret)
